theories/tests/on_val.v
@@ -1,0 +1,65 @@
+From iris.heap_lang Require Import heap.
+From iris.proofmode Require Import tactics.
+
+(* Test proofmode support for [on_val Ψ]. *)
+Section tests.
+  Context `{irisG heap_lang Σ} (Ψ : loc → iProp Σ).
+
+  Goal ∀ v1 v2 P,       (* Using IntoAnd: Destructing pairs. *)
+    (▷ on_val Ψ v1 -∗ ▷ on_val Ψ v2 -∗ P) -∗ on_val Ψ (PairV v1 v2) -∗ P.
+  Proof.
+    iIntros (v1 v2 P) "Hp (Hv1&Hv2)". by iApply ("Hp" with "Hv1 Hv2").
+  Qed.
+
+  Goal ∀ v1 v2 P,       (* Using FromSep: Combining pairs. *)
+    (on_val Ψ (PairV v1 v2) -∗ P) -∗ ▷ on_val Ψ v1 -∗ ▷ on_val Ψ v2 -∗ P.
+  Proof.
+    iIntros (v1 v2 P) "Hp Hv1 Hv2". iCombine "Hv1" "Hv2" as "Hv".
+    by iApply "Hp".
+  Qed.
+
+  Goal ∀ l P,   (* iAssumption, iExact use FromAssumption *)
+    (Ψ l -∗ P) -∗ on_lit Ψ (LitLoc l) -∗ P.
+  Proof. iIntros (l P) "Hp Hlit". by iApply "Hp". Qed.
+
+  Goal ∀ l P,   (* Using FromAssumption transitively *)
+    (Ψ l -∗ P) -∗ on_val Ψ (LitV (LitLoc l)) -∗ P.
+  Proof. iIntros (l P) "Hp Hv". by iApply "Hp". Qed.
+
+  Goal ∀ v P,   (* Using FromAssumption. *)
+    (▷ on_val Ψ v -∗ P) -∗ on_val Ψ (InjLV v) -∗ P.
+  Proof. iIntros (v P) "Hp Hv". by iApply "Hp". Qed.
+
+  Goal ∀ v1 v2 P,       (* Using IntoLater: iNext simplifies the context *)
+    (on_val Ψ v1 ∗ on_val Ψ v2 -∗ P) -∗ on_val Ψ (PairV v1 v2) -∗ ▷ P.
+  Proof. iIntros (v1 v2 P) "Hp Hvi". iNext. by iApply "Hp". Qed.
+
+  Goal ∀ v P,   (* Using IntoLater: iNext simplifies the context *)
+    (on_val Ψ v -∗ P) -∗ on_val Ψ (InjLV v) -∗ ▷ P.
+  Proof. iIntros (v P) "Hp Hv". iNext. by iApply "Hp". Qed.
+
+  Goal ∀ l P,   (* FromAssumption, IntoLater *)
+    (▷ Ψ l -∗ P) -∗ on_val Ψ (InjLV (LitV (LitLoc l))) -∗ P.
+  Proof. iIntros (v P) "Hp Hv". iApply "Hp". by auto. Qed.
+
+  Goal ∀ v P,   (* FromAssumption, IntoLater *)
+    (▷ ▷ on_val Ψ v -∗ P) -∗ on_val Ψ (InjLV (InjRV v)) -∗ P.
+  Proof. iIntros (v P) "Hp Hv". iApply "Hp". by auto. Qed.
+
+  Goal ∀ v1 v2, (* Using FromLater: iNext simplifies the goal *)
+    ▷ (on_val Ψ v1 ∗ on_val Ψ v2) -∗ on_val Ψ (PairV v1 v2).
+  Proof. iIntros (v1 v2) "Hvi". iNext. done. Qed.
+
+  Goal ∀ v,     (* Using FromLater: iNext simplifies the goal *)
+    ▷ on_val Ψ v -∗ on_val Ψ (InjLV v).
+  Proof. iIntros (v) "Hv". iNext. done. Qed.
+
+  Goal ∀ v,     (* Using IsExcept0, except zero *)
+    ◇ on_val Ψ (InjLV v) -∗ on_val Ψ (InjLV v).
+  Proof. iIntros (v) "Hv". by iMod "Hv". Qed.
+
+  Goal ∀ v P,   (* Using IsExcept0, timelessness *)
+    TimelessP P →
+    (P -∗ on_val Ψ (InjLV v)) -∗ ▷ P -∗ on_val Ψ (InjLV v).
+  Proof. iIntros (v P ?) "Hp Hv". iMod "Hv". by iApply "Hp". Qed.
+End tests.
